Weidenbach_Book/CDCL_WNOT.thy
@@ -222,9 +222,9 @@ subsection \<open>More lemmas conflict--propagate and backjumping\<close>
 subsubsection \<open>Termination\<close>
 
 lemma cdcl_cp_normalized_element_all_inv:
-  assumes inv: "cdcl_all_inv_mes S"
+  assumes inv: "cdcl_all_struct_inv S"
   obtains T where "full0 cdcl_cp S T"
-  using assms cdcl_cp_normalized_element unfolding cdcl_all_inv_mes_def by blast
+  using assms cdcl_cp_normalized_element unfolding cdcl_all_struct_inv_def by blast
 
 lemma cdcl_bj_measure:
   assumes "cdcl_bj S T"
@@ -251,7 +251,7 @@ lemma rtranclp_skip_backtrack_backtrack:
   assumes
     "skip\<^sup>*\<^sup>* S T" and
     "backtrack T W" and
-    "cdcl_all_inv_mes S"
+    "cdcl_all_struct_inv S"
   shows "backtrack S W"
   using assms
 proof induction
@@ -279,9 +279,9 @@ next
 
   let ?M =  "Propagated L' C' # M"
   have "cdcl\<^sup>*\<^sup>* S T" using bj cdcl_bj.skip mono_rtranclp[of skip cdcl S T] other st by meson
-  hence inv': "cdcl_all_inv_mes T"
-    using rtranclp_cdcl_all_inv_mes_inv inv by blast
-  have M_lev: "cdcl_M_level_inv T" using inv' unfolding cdcl_all_inv_mes_def by auto
+  hence inv': "cdcl_all_struct_inv T"
+    using rtranclp_cdcl_all_struct_inv_inv inv by blast
+  have M_lev: "cdcl_M_level_inv T" using inv' unfolding cdcl_all_struct_inv_def by auto
   hence n_d': "no_dup ?M"
     using T unfolding cdcl_M_level_inv_def by auto
 
@@ -294,7 +294,7 @@ next
   have L'_M: "atm_of L' \<notin> atm_of ` lits_of M"
     using n_d' unfolding lits_of_def by auto
   have "?M \<Turnstile>as CNot ?D"
-    using inv' T unfolding cdcl_conflicting_def cdcl_all_inv_mes_def by auto
+    using inv' T unfolding cdcl_conflicting_def cdcl_all_struct_inv_def by auto
   hence "L' \<notin># ?D"
     using L_L' L'_M unfolding true_annots_def by (auto simp add: true_annot_def true_cls_def
       atm_of_in_atm_of_set_iff_in_set_or_uminus_in_set Ball_mset_def
@@ -349,7 +349,7 @@ lemma rtranclp_skip_backtrack_backtrack_end:
   assumes
     skip: "skip\<^sup>*\<^sup>* S T" and
     bt: "backtrack S W" and
-    inv: "cdcl_all_inv_mes S"
+    inv: "cdcl_all_struct_inv S"
   shows "backtrack T W"
   using assms
 proof -
@@ -374,11 +374,11 @@ proof -
       conflicting_update_trial delete_trail_and_rebuild.simps init_clss_append_trail
       init_clss_update_trial learned_clss_append_trail learned_clss_update_trial old.prod.inject
       state_eq_backtrack_lvl state_eq_conflicting state_eq_init_clss state_eq_learned_clss)
-  have "cdcl_all_inv_mes T"
-    apply (rule rtranclp_cdcl_all_inv_mes_inv[OF _ inv])
+  have "cdcl_all_struct_inv T"
+    apply (rule rtranclp_cdcl_all_struct_inv_inv[OF _ inv])
     using bj cdcl_bj.skip local.skip other rtranclp_mono[of skip cdcl] by blast
   hence "M\<^sub>T \<Turnstile>as CNot ?D"
-    unfolding cdcl_all_inv_mes_def cdcl_conflicting_def using T by blast
+    unfolding cdcl_all_struct_inv_def cdcl_conflicting_def using T by blast
   have "\<forall>L\<in>#?D. atm_of L \<in> atm_of ` lits_of M\<^sub>T"
     proof -
       have f1: "\<And>l. \<not> M\<^sub>T \<Turnstile>a {#- l#} \<or> atm_of l \<in> atm_of ` lits_of M\<^sub>T"
@@ -390,7 +390,7 @@ proof -
         using f1 by (meson \<open>M\<^sub>T \<Turnstile>as CNot (D + {#L#})\<close> ball_msetI true_annots_CNot_all_atms_defined)
     qed
   moreover have "no_dup M"
-    using inv S unfolding cdcl_all_inv_mes_def cdcl_M_level_inv_def by auto
+    using inv S unfolding cdcl_all_struct_inv_def cdcl_M_level_inv_def by auto
   ultimately have "\<forall>L\<in>#?D. atm_of L \<notin> atm_of ` lits_of MS"
     unfolding M unfolding lits_of_def by auto
   hence H: "\<And>L. L\<in>#?D \<Longrightarrow> get_level L M  = get_level L M\<^sub>T"
@@ -469,7 +469,7 @@ lemma backtrack_unique:
   assumes
     bt_T: "backtrack S T" and
     bt_U: "backtrack S U" and
-    inv: "cdcl_all_inv_mes S"
+    inv: "cdcl_all_struct_inv S"
   shows "T \<sim> U"
 proof -
   obtain M N U' k D L i K M1 M2 where
@@ -494,7 +494,7 @@ proof -
   obtain c' where M': "M = c' @ M2' @ Marked K' (i' + 1) # M1'"
     using decomp' by auto
   have marked: "get_all_levels_of_marked M = rev [1..<1+k]"
-    using inv S unfolding cdcl_all_inv_mes_def cdcl_M_level_inv_def by auto
+    using inv S unfolding cdcl_all_struct_inv_def cdcl_M_level_inv_def by auto
   hence "i < k"
     unfolding M
     by (force simp add: rev_swap[symmetric] dest!: arg_cong[of _ _ set])
@@ -537,7 +537,7 @@ lemma if_can_apply_backtrack_no_more_resolve:
   assumes
     skip: "skip\<^sup>*\<^sup>* S U" and
     bt: "backtrack S T" and
-    inv: "cdcl_all_inv_mes S"
+    inv: "cdcl_all_struct_inv S"
   shows "\<not>resolve U V"
 proof (rule ccontr)
   assume resolve: "\<not>\<not>resolve U V"
@@ -570,7 +570,7 @@ proof (rule ccontr)
   obtain c where M: "M' = c @ M2 @ Marked K (i + 1) # M1"
     using get_all_marked_decomposition_exists_prepend[OF decomp] by auto
   have marked: "get_all_levels_of_marked M' = rev [1..<1+k]"
-    using inv S' unfolding cdcl_all_inv_mes_def cdcl_M_level_inv_def by auto
+    using inv S' unfolding cdcl_all_struct_inv_def cdcl_M_level_inv_def by auto
   hence "i < k"
     unfolding M by (force simp add: rev_swap[symmetric] dest!: arg_cong[of _ _ set])
 
@@ -586,11 +586,11 @@ proof (rule ccontr)
         have M': "M' = M\<^sub>0 @ Propagated L ( (C + {#L#})) # M"
           using tr_S U S S' by (auto simp: lits_of_def)
         have "no_dup M'"
-           using inv U S' unfolding cdcl_all_inv_mes_def cdcl_M_level_inv_def by auto
+           using inv U S' unfolding cdcl_all_struct_inv_def cdcl_M_level_inv_def by auto
         have atm_L_notin_M: "atm_of L \<notin> atm_of ` (lits_of M)"
           using \<open>no_dup M'\<close> M' U S S' by (auto simp: lits_of_def)
         have "get_all_levels_of_marked M' = rev [1..<1+k]"
-          using inv U S' unfolding cdcl_all_inv_mes_def cdcl_M_level_inv_def by auto
+          using inv U S' unfolding cdcl_all_struct_inv_def cdcl_M_level_inv_def by auto
         hence "get_all_levels_of_marked M = rev [1..<1+k]"
           using nm M' S' U by (simp add: get_all_levels_of_marked_no_marked)
         hence get_lev_L:
@@ -611,10 +611,10 @@ proof (rule ccontr)
   have [simp]: "D = D'" using DD' by auto
   have "cdcl\<^sup>*\<^sup>* S U"
     using bj cdcl_bj.skip local.skip mono_rtranclp[of skip cdcl S U] other by meson
-  hence "cdcl_all_inv_mes U"
-    using inv rtranclp_cdcl_all_inv_mes_inv by blast
+  hence "cdcl_all_struct_inv U"
+    using inv rtranclp_cdcl_all_struct_inv_inv by blast
   hence "Propagated L ( (C + {#L#})) # M \<Turnstile>as CNot (D' + {#L'#})"
-    using cdcl_all_inv_mes_def cdcl_conflicting_def U by auto
+    using cdcl_all_struct_inv_def cdcl_conflicting_def U by auto
   hence "\<forall>L'\<in>#D. atm_of L' \<in> atm_of ` lits_of (Propagated L ( (C + {#L#})) # M)"
     by (metis CNot_plus CNot_singleton Un_insert_right \<open>D = D'\<close> true_annots_insert ball_msetI
       atm_of_in_atm_of_set_iff_in_set_or_uminus_in_set  in_CNot_implies_uminus(2)
@@ -634,7 +634,7 @@ lemma if_can_apply_resolve_no_more_backtrack:
   assumes
     skip: "skip\<^sup>*\<^sup>* S U" and
     resolve: "resolve S T" and
-    inv: "cdcl_all_inv_mes S"
+    inv: "cdcl_all_struct_inv S"
   shows "\<not>backtrack U V"
   using assms
   by (meson if_can_apply_backtrack_no_more_resolve rtranclp.rtrancl_refl
@@ -644,13 +644,13 @@ lemma if_can_apply_backtrack_skip_or_resolve_is_skip:
   assumes
     bt: "backtrack S T" and
     skip: "skip_or_resolve\<^sup>*\<^sup>* S U" and
-    inv: "cdcl_all_inv_mes S"
+    inv: "cdcl_all_struct_inv S"
   shows "skip\<^sup>*\<^sup>* S U"
   using assms(2,3,1)
   by induction (simp_all add: if_can_apply_backtrack_no_more_resolve)
 
 lemma cdcl_bj_bj_decomp:
-  assumes "cdcl_bj\<^sup>*\<^sup>* S W" and "cdcl_all_inv_mes S"
+  assumes "cdcl_bj\<^sup>*\<^sup>* S W" and "cdcl_all_struct_inv S"
   shows
     "(\<exists>T U V. (\<lambda>S T. skip_or_resolve S T \<and> no_step backtrack S)\<^sup>*\<^sup>* S T
         \<and> (\<lambda>T U. resolve T U \<and> no_step backtrack T) T U
@@ -670,7 +670,7 @@ next
   hence IH: "?R S W \<or> ?S S W" using IH by blast
 
   have "cdcl\<^sup>*\<^sup>* S W" by (metis cdcl_o.bj mono_rtranclp other st)
-  hence inv_W: "cdcl_all_inv_mes W" by (simp add: rtranclp_cdcl_all_inv_mes_inv step.prems)
+  hence inv_W: "cdcl_all_struct_inv W" by (simp add: rtranclp_cdcl_all_struct_inv_inv step.prems)
   consider
       (BT) X' where "backtrack W X'"
     | (skip) "no_step backtrack W" and "skip W X"
@@ -711,13 +711,13 @@ next
             using  RS(1) cdcl_bj.resolve cdcl_o.bj  other skip
             mono_rtranclp[of " (\<lambda>S T. skip_or_resolve S T \<and> no_step backtrack S)" cdcl S T]
             by meson
-          hence "cdcl_all_inv_mes U"
-            by (meson RS(2) cdcl_all_inv_mes_inv cdcl_bj.resolve cdcl_o.bj other
-              rtranclp_cdcl_all_inv_mes_inv step.prems)
+          hence "cdcl_all_struct_inv U"
+            by (meson RS(2) cdcl_all_struct_inv_inv cdcl_bj.resolve cdcl_o.bj other
+              rtranclp_cdcl_all_struct_inv_inv step.prems)
           { fix U'
             assume "skip\<^sup>*\<^sup>* U U'" and "skip\<^sup>*\<^sup>* U' W"
-            have "cdcl_all_inv_mes U'"
-              using \<open>cdcl_all_inv_mes U\<close> \<open>skip\<^sup>*\<^sup>* U U'\<close> rtranclp_cdcl_all_inv_mes_inv
+            have "cdcl_all_struct_inv U'"
+              using \<open>cdcl_all_struct_inv U\<close> \<open>skip\<^sup>*\<^sup>* U U'\<close> rtranclp_cdcl_all_struct_inv_inv
                  cdcl_o.bj rtranclp_mono[of skip cdcl] other skip by blast
             hence "no_step backtrack U'"
               using if_can_apply_backtrack_no_more_resolve[OF \<open>skip\<^sup>*\<^sup>* U' W\<close> ] res by blast
@@ -767,8 +767,8 @@ next
             assume "skip\<^sup>*\<^sup>* S U'" and "skip\<^sup>*\<^sup>* U' W"
             hence "cdcl\<^sup>*\<^sup>* S U'"
               using mono_rtranclp[of skip cdcl S U'] by (simp add: cdcl_o.bj other skip)
-            hence "cdcl_all_inv_mes U'"
-              by (metis (no_types, hide_lams) \<open>cdcl_all_inv_mes S\<close> rtranclp_cdcl_all_inv_mes_inv)
+            hence "cdcl_all_struct_inv U'"
+              by (metis (no_types, hide_lams) \<open>cdcl_all_struct_inv S\<close> rtranclp_cdcl_all_struct_inv_inv)
             hence "no_step backtrack U'"
               using if_can_apply_backtrack_no_more_resolve[OF \<open>skip\<^sup>*\<^sup>* U' W\<close> ] res by blast
           }
@@ -821,7 +821,7 @@ lemma cdcl_bj_strongly_confluent:
      "cdcl_bj\<^sup>*\<^sup>* S V" and
      "cdcl_bj\<^sup>*\<^sup>* S T" and
      n_s: "no_step cdcl_bj V" and
-     inv: "cdcl_all_inv_mes S"
+     inv: "cdcl_all_struct_inv S"
    shows "T \<sim> V \<or> cdcl_bj\<^sup>*\<^sup>* T V"
    using assms(2)
 proof induction
@@ -847,8 +847,8 @@ next
         using IH n_s s_o_r by (metis rtranclp_unfold tranclpD)
       have "cdcl\<^sup>*\<^sup>* S T"
         by (metis (no_types, hide_lams) bj mono_rtranclp[of cdcl_bj cdcl] other st)
-      hence inv_T: "cdcl_all_inv_mes T"
-        by (metis (no_types, hide_lams) inv rtranclp_cdcl_all_inv_mes_inv)
+      hence inv_T: "cdcl_all_struct_inv T"
+        by (metis (no_types, hide_lams) inv rtranclp_cdcl_all_struct_inv_inv)
 
       show ?thesis
         using s_o_r
@@ -902,7 +902,7 @@ lemma cdcl_bj_unique_normal_form:
     ST: "cdcl_bj\<^sup>*\<^sup>* S T" and SU: "cdcl_bj\<^sup>*\<^sup>* S U" and
     n_s_U: "no_step cdcl_bj U" and
     n_s_T: "no_step cdcl_bj T" and
-    inv: "cdcl_all_inv_mes S"
+    inv: "cdcl_all_struct_inv S"
   shows "T \<sim> U"
 proof -
   have "T \<sim> U \<or> cdcl_bj\<^sup>*\<^sup>* T U"
@@ -913,7 +913,7 @@ qed
 
 lemma full0_cdcl_bj_unique_normal_form:
  assumes "full0 cdcl_bj S T" and "full0 cdcl_bj S U" and
-   inv: "cdcl_all_inv_mes S"
+   inv: "cdcl_all_struct_inv S"
  shows "T \<sim> U"
    using cdcl_bj_unique_normal_form assms unfolding full0_def by blast
 
@@ -1008,7 +1008,7 @@ lemma reduce_trail_to_length:
 
 lemma cdcl_fw_is_cdcl\<^sub>N\<^sub>O\<^sub>T_merged:
   assumes
-    inv: "cdcl_all_inv_mes S" and
+    inv: "cdcl_all_struct_inv S" and
     cdcl:"cdcl_fw S T"
   shows "cdcl\<^sub>N\<^sub>O\<^sub>T_merged S T
     \<or> (no_step cdcl_fw T \<and> conflicting T \<noteq> C_True)"
@@ -1039,7 +1039,7 @@ next
   have "decide\<^sub>N\<^sub>O\<^sub>T S T"
     apply (rule decide\<^sub>N\<^sub>O\<^sub>T.decide\<^sub>N\<^sub>O\<^sub>T)
        using undef_L apply simp
-     using atm_L inv unfolding cdcl_all_inv_mes_def no_strange_atm_def clauses_def apply auto[]
+     using atm_L inv unfolding cdcl_all_struct_inv_def no_strange_atm_def clauses_def apply auto[]
     using T unfolding state_eq_def state_eq\<^sub>N\<^sub>O\<^sub>T_def by (auto simp: clauses_def)
   then show ?case using cdcl\<^sub>N\<^sub>O\<^sub>T_merged_decide\<^sub>N\<^sub>O\<^sub>T by blast
 next
@@ -1053,7 +1053,7 @@ next
      T: "T \<sim> remove_cls C S"
     by auto
   have "init_clss S \<Turnstile>pm C"
-    using inv C_le unfolding cdcl_all_inv_mes_def cdcl_learned_clause_def
+    using inv C_le unfolding cdcl_all_struct_inv_def cdcl_learned_clause_def
     by (meson mem_set_mset_iff true_clss_clss_in_imp_true_clss_cls)
   then have S_C: "clauses S - replicate_mset (count (clauses S) C) C \<Turnstile>pm C"
     using C_init C_le unfolding clauses_def by (simp add: Un_Diff)
@@ -1117,23 +1117,23 @@ next
             using s_o_r by auto
           then show ?case using IH by auto
         qed
-      have inv_T: "cdcl_all_inv_mes T"
-        by (meson cdcl_cp.simps confl inv r_into_rtranclp rtranclp_cdcl_all_inv_mes_inv
+      have inv_T: "cdcl_all_struct_inv T"
+        by (meson cdcl_cp.simps confl inv r_into_rtranclp rtranclp_cdcl_all_struct_inv_inv
           rtranclp_cdcl_cp_rtranclp_cdcl)
       have "cdcl\<^sup>*\<^sup>* T T'"
         using rtranclp_skip_or_resolve_rtranclp_cdcl s_or_r by blast
-      have inv_T': "cdcl_all_inv_mes T'"
-        using \<open>cdcl\<^sup>*\<^sup>* T T'\<close> inv_T rtranclp_cdcl_all_inv_mes_inv by blast
-      have inv_U: "cdcl_all_inv_mes U"
-        using cdcl_fw_restart_cdcl confl fw_r_conflict inv local.bj rtranclp_cdcl_all_inv_mes_inv
+      have inv_T': "cdcl_all_struct_inv T'"
+        using \<open>cdcl\<^sup>*\<^sup>* T T'\<close> inv_T rtranclp_cdcl_all_struct_inv_inv by blast
+      have inv_U: "cdcl_all_struct_inv U"
+        using cdcl_fw_restart_cdcl confl fw_r_conflict inv local.bj rtranclp_cdcl_all_struct_inv_inv
         by blast
       then have undef_L: "undefined_lit L (tl (trail U))"
-        using U unfolding cdcl_all_inv_mes_def cdcl_M_level_inv_def by (auto simp: defined_lit_map)
+        using U unfolding cdcl_all_struct_inv_def cdcl_M_level_inv_def by (auto simp: defined_lit_map)
       have [simp]: "init_clss S = init_clss T'"
         using \<open>cdcl\<^sup>*\<^sup>* T T'\<close> cdcl_init_clss confl by (auto dest!: cdcl_init_clss cdcl.conflict
           rtranclp_cdcl_init_clss)
       then have atm_L: "atm_of L \<in> atms_of_mu (clauses S)"
-        using inv_T' confl_T' unfolding cdcl_all_inv_mes_def no_strange_atm_def clauses_def by auto
+        using inv_T' confl_T' unfolding cdcl_all_struct_inv_def no_strange_atm_def clauses_def by auto
       obtain M where tr_T: "trail T = M @ trail T'"
         using s_or_r by (induction rule: rtranclp_induct) auto
       obtain M' where
@@ -1144,7 +1144,7 @@ next
         have tr_T: "trail S = M'' @  Marked K (i+1) # tl (trail U)"
         using tr_T tr_T' confl unfolding M''_def by auto
       have "init_clss T' + learned_clss S \<Turnstile>pm D + {#L#}"
-        using inv_T' confl_T' unfolding cdcl_all_inv_mes_def cdcl_learned_clause_def clauses_def
+        using inv_T' confl_T' unfolding cdcl_all_struct_inv_def cdcl_learned_clause_def clauses_def
         by simp
       have "reduce_trail_to (convert_trail_from_NOT (convert_trail_from_W M1)) S =
         reduce_trail_to M1 S"
@@ -1158,13 +1158,13 @@ next
       ultimately have [simp]: "trail (reduce_trail_to\<^sub>N\<^sub>O\<^sub>T (convert_trail_from_W M1) S) = M1"
         using M1_M2 confl by (auto simp add: reduce_trail_to\<^sub>N\<^sub>O\<^sub>T_reduce_trail_convert)
       have "every_mark_is_a_conflict U"
-        using inv_U unfolding cdcl_all_inv_mes_def cdcl_conflicting_def by simp
+        using inv_U unfolding cdcl_all_struct_inv_def cdcl_conflicting_def by simp
       then have "tl (trail U) \<Turnstile>as CNot D"
         by (metis add_diff_cancel_left' append_self_conv2 tr_U union_commute)
       have "backjump_l S U"
         apply (rule backjump_l)
                 using tr_T apply simp
-               using inv unfolding cdcl_all_inv_mes_def cdcl_M_level_inv_def apply simp
+               using inv unfolding cdcl_all_struct_inv_def cdcl_M_level_inv_def apply simp
                using U M1_M2 confl apply (auto elim!:  simp: state_eq\<^sub>N\<^sub>O\<^sub>T_def
                simp del: state_simp\<^sub>N\<^sub>O\<^sub>T)[]
               using C\<^sub>S apply simp
@@ -1173,9 +1173,9 @@ next
             using undef_L apply simp
            using atm_L apply simp
           using \<open>init_clss T' + learned_clss S \<Turnstile>pm D + {#L#}\<close> unfolding clauses_def apply simp
-         using \<open>tl (trail U) \<Turnstile>as CNot D\<close> inv_T' unfolding cdcl_all_inv_mes_def distinct_cdcl_state_def
+         using \<open>tl (trail U) \<Turnstile>as CNot D\<close> inv_T' unfolding cdcl_all_struct_inv_def distinct_cdcl_state_def
          apply simp
-        using \<open>tl (trail U) \<Turnstile>as CNot D\<close> inv_T' inv_U U confl_T' unfolding cdcl_all_inv_mes_def distinct_cdcl_state_def
+        using \<open>tl (trail U) \<Turnstile>as CNot D\<close> inv_T' inv_U U confl_T' unfolding cdcl_all_struct_inv_def distinct_cdcl_state_def
         apply simp_all
         done
       then show ?thesis using cdcl\<^sub>N\<^sub>O\<^sub>T_merged_backjump_l by fast
@@ -1186,7 +1186,7 @@ abbreviation cdcl\<^sub>N\<^sub>O\<^sub>T_restart where
 "cdcl\<^sub>N\<^sub>O\<^sub>T_restart \<equiv> restart_ops.cdcl\<^sub>N\<^sub>O\<^sub>T_with_restarts cdcl\<^sub>N\<^sub>O\<^sub>T restart"
 lemma cdcl_fw_restart_is_cdcl\<^sub>N\<^sub>O\<^sub>T_merged_restart_no_step:
   assumes
-    inv: "cdcl_all_inv_mes S" and
+    inv: "cdcl_all_struct_inv S" and
     cdcl:"cdcl_fw_restart S T"
   shows "cdcl\<^sub>N\<^sub>O\<^sub>T_restart\<^sup>*\<^sup>* S T \<or> (no_step cdcl_fw T \<and> conflicting T \<noteq> C_True)"
 proof -
@@ -1201,7 +1201,7 @@ proof -
       then have "cdcl\<^sub>N\<^sub>O\<^sub>T_merged S T \<or> (no_step cdcl_fw T \<and> conflicting T \<noteq> C_True)"
         using inv cdcl_fw_is_cdcl\<^sub>N\<^sub>O\<^sub>T_merged by blast
       moreover have "inv\<^sub>N\<^sub>O\<^sub>T S"
-        using inv unfolding cdcl_all_inv_mes_def cdcl_M_level_inv_def by auto
+        using inv unfolding cdcl_all_struct_inv_def cdcl_M_level_inv_def by auto
       ultimately show ?thesis
         using cdcl\<^sub>N\<^sub>O\<^sub>T_merged_is_tranclp_cdcl\<^sub>N\<^sub>O\<^sub>T rtranclp_cdcl\<^sub>N\<^sub>O\<^sub>T_merged_is_rtranclp_cdcl\<^sub>N\<^sub>O\<^sub>T_and_inv
         rtranclp_mono[of cdcl\<^sub>N\<^sub>O\<^sub>T cdcl\<^sub>N\<^sub>O\<^sub>T_restart]
@@ -1217,17 +1217,17 @@ abbreviation \<mu>\<^sub>F\<^sub>W :: "'st \<Rightarrow> nat" where
 
 lemma cdcl_fw_\<mu>\<^sub>F\<^sub>W_decreasing:
   assumes
-    inv: "cdcl_all_inv_mes S" and
+    inv: "cdcl_all_struct_inv S" and
     fw: "cdcl_fw S T"
   shows "\<mu>\<^sub>F\<^sub>W T < \<mu>\<^sub>F\<^sub>W S"
 proof -
   let ?A = "init_clss S"
   have atm_clauses: "atms_of_mu (clauses S) \<subseteq> atms_of_mu ?A"
-    using inv unfolding cdcl_all_inv_mes_def no_strange_atm_def clauses_def by auto
+    using inv unfolding cdcl_all_struct_inv_def no_strange_atm_def clauses_def by auto
   have atm_trail: "atm_of ` lits_of (trail S) \<subseteq> atms_of_mu ?A"
-    using inv unfolding cdcl_all_inv_mes_def no_strange_atm_def clauses_def by auto
+    using inv unfolding cdcl_all_struct_inv_def no_strange_atm_def clauses_def by auto
   have n_d: "no_dup (trail S)"
-    using inv unfolding cdcl_all_inv_mes_def by auto
+    using inv unfolding cdcl_all_struct_inv_def by auto
   have [simp]: "\<not> no_step cdcl_fw S"
     using fw by auto
   have [simp]: "init_clss S = init_clss T"
@@ -1249,34 +1249,34 @@ proof -
     qed
 qed
 
-lemma wf_cdcl_fw: "wf {(T, S). cdcl_all_inv_mes S \<and> cdcl_fw S T}"
+lemma wf_cdcl_fw: "wf {(T, S). cdcl_all_struct_inv S \<and> cdcl_fw S T}"
   apply (rule wfP_if_measure[of _ _ "\<mu>\<^sub>F\<^sub>W"])
   using cdcl_fw_\<mu>\<^sub>F\<^sub>W_decreasing by blast
 
-lemma cdcl_all_inv_mes_tranclp_cdcl_fw_tranclp_cdcl_fw_cdcl_all_inv_mes:
+lemma cdcl_all_struct_inv_tranclp_cdcl_fw_tranclp_cdcl_fw_cdcl_all_struct_inv:
   assumes
-    inv: "cdcl_all_inv_mes b"
+    inv: "cdcl_all_struct_inv b"
     "cdcl_fw\<^sup>+\<^sup>+ b a"
-  shows "(\<lambda>S T. cdcl_all_inv_mes S \<and> cdcl_fw S T)\<^sup>+\<^sup>+ b a"
+  shows "(\<lambda>S T. cdcl_all_struct_inv S \<and> cdcl_fw S T)\<^sup>+\<^sup>+ b a"
   using assms(2)
 proof induction
   case base
   then show ?case using inv by auto
 next
   case (step c d) note st =this(1) and fw = this(2) and IH = this(3)
-  have "cdcl_all_inv_mes c"
+  have "cdcl_all_struct_inv c"
     using tranclp_into_rtranclp[OF st] cdcl_fw_rtranclp_cdcl
-    assms(1) rtranclp_cdcl_all_inv_mes_inv rtranclp_mono[of cdcl_fw "cdcl\<^sup>*\<^sup>*"] by fastforce
-  then have "(\<lambda>S T. cdcl_all_inv_mes S \<and> cdcl_fw S T)\<^sup>+\<^sup>+ c d"
+    assms(1) rtranclp_cdcl_all_struct_inv_inv rtranclp_mono[of cdcl_fw "cdcl\<^sup>*\<^sup>*"] by fastforce
+  then have "(\<lambda>S T. cdcl_all_struct_inv S \<and> cdcl_fw S T)\<^sup>+\<^sup>+ c d"
     using fw by auto
   then show ?case using IH by auto
 qed
 
-lemma wf_tranclp_cdcl_fw: "wf {(T, S). cdcl_all_inv_mes S \<and> cdcl_fw\<^sup>+\<^sup>+ S T}"
+lemma wf_tranclp_cdcl_fw: "wf {(T, S). cdcl_all_struct_inv S \<and> cdcl_fw\<^sup>+\<^sup>+ S T}"
   using wf_trancl[OF wf_cdcl_fw]
   apply (rule wf_subset)
   by (auto simp: trancl_set_tranclp
-    cdcl_all_inv_mes_tranclp_cdcl_fw_tranclp_cdcl_fw_cdcl_all_inv_mes)
+    cdcl_all_struct_inv_tranclp_cdcl_fw_tranclp_cdcl_fw_cdcl_all_struct_inv)
 
 lemma backtrack_is_full_cdcl_bj:
   assumes bt: "backtrack S T"
@@ -1494,7 +1494,7 @@ lemma cdcl_cp_cdcl_bj_bissimulation:
   assumes
     "full0 cdcl_cp T U" and
     "cdcl_bj\<^sup>*\<^sup>* T T'" and
-    "cdcl_all_inv_mes T" and
+    "cdcl_all_struct_inv T" and
     "no_step cdcl_bj T'"
   shows "full0 cdcl_cp T' U
     \<or> (\<exists>U' U''. full0 cdcl_cp T' U'' \<and> full cdcl_bj U U' \<and> full0 cdcl_cp U' U'' \<and> cdcl_s'\<^sup>*\<^sup>* U U'')"
@@ -1508,8 +1508,8 @@ next
   have "cdcl\<^sup>*\<^sup>* T T''"
     by (metis (no_types, lifting) cdcl_o.bj local.bj mono_rtranclp[of cdcl_bj cdcl T T''] other st
       rtranclp.rtrancl_into_rtrancl)
-  hence inv_T'': "cdcl_all_inv_mes T''"
-    using inv rtranclp_cdcl_all_inv_mes_inv by blast
+  hence inv_T'': "cdcl_all_struct_inv T''"
+    using inv rtranclp_cdcl_all_struct_inv_inv by blast
   have "cdcl_bj\<^sup>+\<^sup>+ T T''"
     using local.bj st by auto
   have "full cdcl_bj T T''"
@@ -1550,7 +1550,7 @@ lemma cdcl_cp_cdcl_bj_bissimulation':
   assumes
     "full0 cdcl_cp T U" and
     "cdcl_bj\<^sup>*\<^sup>* T T'" and
-    "cdcl_all_inv_mes T" and
+    "cdcl_all_struct_inv T" and
     "no_step cdcl_bj T'"
   shows "full0 cdcl_cp T' U
     \<or> (\<exists>U'. full cdcl_bj U U' \<and> (\<forall>U''. full0 cdcl_cp U' U'' \<longrightarrow> full0 cdcl_cp T' U''
@@ -1565,8 +1565,8 @@ next
   have "cdcl\<^sup>*\<^sup>* T T''"
     by (metis (no_types, lifting) cdcl_o.bj local.bj mono_rtranclp[of cdcl_bj cdcl T T''] other st
       rtranclp.rtrancl_into_rtrancl)
-  hence inv_T'': "cdcl_all_inv_mes T''"
-    using inv rtranclp_cdcl_all_inv_mes_inv by blast
+  hence inv_T'': "cdcl_all_struct_inv T''"
+    using inv rtranclp_cdcl_all_struct_inv_inv by blast
   have "cdcl_bj\<^sup>+\<^sup>+ T T''"
     using local.bj st by auto
   have "full cdcl_bj T T''"
@@ -1668,7 +1668,7 @@ next
 qed
 
 lemma cdcl_s_cdcl_s'_connected:
-  assumes "cdcl_s S U" and "cdcl_all_inv_mes S"
+  assumes "cdcl_s S U" and "cdcl_all_struct_inv S"
   shows "cdcl_s' S U
     \<or> (\<exists>U'. full cdcl_bj U U' \<and> (\<forall>U''. full0 cdcl_cp U' U'' \<longrightarrow> cdcl_s' S U'' ))"
   using assms
@@ -1687,8 +1687,8 @@ next
       thus ?thesis using cdcl_s'.simps full n_s by blast
     next
       case bj
-      have inv_T: "cdcl_all_inv_mes T"
-        using cdcl_all_inv_mes_inv o other other'.prems by blast
+      have inv_T: "cdcl_all_struct_inv T"
+        using cdcl_all_struct_inv_inv o other other'.prems by blast
       consider
           (cp) "full0 cdcl_cp T U" and "no_step cdcl_bj T"
         | (fbj) T' where "full cdcl_bj T T'"
@@ -1724,7 +1724,7 @@ next
 qed
 
 lemma cdcl_s_cdcl_s'_connected':
-  assumes "cdcl_s S U" and "cdcl_all_inv_mes S"
+  assumes "cdcl_s S U" and "cdcl_all_struct_inv S"
   shows "cdcl_s' S U
     \<or> (\<exists>U' U''. cdcl_s' S U'' \<and> full cdcl_bj U U' \<and> full0 cdcl_cp U' U'')"
   using assms
@@ -1756,8 +1756,8 @@ next
         qed
       have "cdcl_bj\<^sup>*\<^sup>* T T'"
         using T' unfolding full0_def by simp
-      have "cdcl_all_inv_mes T"
-        using cdcl_all_inv_mes_inv o other other'.prems by blast
+      have "cdcl_all_struct_inv T"
+        using cdcl_all_struct_inv_inv o other other'.prems by blast
       then consider
           (T'U) "full0 cdcl_cp T' U"
         | (U) U' U'' where
@@ -1784,7 +1784,7 @@ next
 qed
 
 lemma cdcl_s_cdcl_s'_no_step:
-  assumes "cdcl_s S U" and "cdcl_all_inv_mes S" and "no_step cdcl_bj U"
+  assumes "cdcl_s S U" and "cdcl_all_struct_inv S" and "no_step cdcl_bj U"
   shows "cdcl_s' S U"
   using cdcl_s_cdcl_s'_connected[OF assms(1,2)] assms(3)
   by (metis (no_types, lifting) full_def tranclpD)
@@ -1905,7 +1905,7 @@ next
 qed
 
 lemma n_step_cdcl_s_iff_no_step_cdcl_cl_cdcl_o:
-  assumes inv: "cdcl_all_inv_mes S"
+  assumes inv: "cdcl_all_struct_inv S"
   shows "no_step cdcl_s' S \<longleftrightarrow> no_step cdcl_cp S \<and> no_step cdcl_o S" (is "?S' S \<longleftrightarrow> ?C S \<and> ?O S")
 proof
   assume "?C S \<and> ?O S"
@@ -1929,8 +1929,8 @@ next
         by auto
       then obtain T where "full cdcl_cp S' T"
         using cdcl_cp_normalized_element_all_inv inv
-        by (meson cdcl_all_inv_mes_def cdcl_s_cdcl_s'_connected' cdcl_then_exists_cdcl_s_step n_s)
-      thus False using n_s by (meson \<open>cdcl_o S S'\<close> cdcl_all_inv_mes_def cdcl_s_cdcl_s'_connected'
+        by (meson cdcl_all_struct_inv_def cdcl_s_cdcl_s'_connected' cdcl_then_exists_cdcl_s_step n_s)
+      thus False using n_s by (meson \<open>cdcl_o S S'\<close> cdcl_all_struct_inv_def cdcl_s_cdcl_s'_connected'
         cdcl_then_exists_cdcl_s_step inv)
     qed
   ultimately show "?C S \<and> ?O S" by auto
@@ -1974,14 +1974,14 @@ lemma rtranclp_cdcl_s'_rtranclp_cdcl:
   using rtranclp_unfold[of cdcl_s' S S'] tranclp_cdcl_s'_tranclp_cdcl[of S S'] by auto
 
 lemma full0_cdcl_s_iff_full0_cdcl_s':
-  assumes inv: "cdcl_all_inv_mes S"
+  assumes inv: "cdcl_all_struct_inv S"
   shows "full0 cdcl_s S T \<longleftrightarrow> full0 cdcl_s' S T" (is "?S \<longleftrightarrow> ?S'")
 proof
   assume ?S'
   hence "cdcl\<^sup>*\<^sup>* S T"
     using rtranclp_cdcl_s'_rtranclp_cdcl[of S T] unfolding full0_def by blast
-  hence inv': "cdcl_all_inv_mes T"
-    using rtranclp_cdcl_all_inv_mes_inv inv by blast
+  hence inv': "cdcl_all_struct_inv T"
+    using rtranclp_cdcl_all_struct_inv_inv inv by blast
   have "cdcl_s\<^sup>*\<^sup>* S T"
     using \<open>?S'\<close> unfolding full0_def
       using cdcl_s'_is_rtranclp_cdcl_s rtranclp_mono[of cdcl_s' "cdcl_s\<^sup>*\<^sup>*"] by auto
@@ -1989,8 +1989,8 @@ proof
     using \<open>?S'\<close> inv' cdcl_s_cdcl_s'_connected' unfolding full0_def by blast
 next
   assume ?S
-  hence inv_T:"cdcl_all_inv_mes T"
-    by (metis assms full0_def rtranclp_cdcl_all_inv_mes_inv rtranclp_cdcl_s_rtranclp_cdcl)
+  hence inv_T:"cdcl_all_struct_inv T"
+    by (metis assms full0_def rtranclp_cdcl_all_struct_inv_inv rtranclp_cdcl_s_rtranclp_cdcl)
 
   consider
       (s')  "cdcl_s'\<^sup>*\<^sup>* S T"
@@ -2001,7 +2001,7 @@ next
     proof cases
       case s'
       thus ?thesis
-        by (metis \<open>full0 cdcl_s S T\<close> inv_T cdcl_all_inv_mes_def cdcl_s'.simps cdcl_s.conflict'
+        by (metis \<open>full0 cdcl_s S T\<close> inv_T cdcl_all_struct_inv_def cdcl_s'.simps cdcl_s.conflict'
           cdcl_then_exists_cdcl_s_step full0_def n_step_cdcl_s_iff_no_step_cdcl_cl_cdcl_o)
     next
       case (st S')
@@ -2009,7 +2009,7 @@ next
         using conflicting_clause_full0_cdcl_cp st(3) by blast
       moreover
         have n_s: "no_step cdcl_bj T"
-          by (metis \<open>full0 cdcl_s S T\<close> bj inv_T cdcl_all_inv_mes_def cdcl_then_exists_cdcl_s_step
+          by (metis \<open>full0 cdcl_s S T\<close> bj inv_T cdcl_all_struct_inv_def cdcl_then_exists_cdcl_s_step
             full0_def)
         hence "full cdcl_bj S' T"
           using st(2) unfolding full_def by blast
@@ -2020,7 +2020,7 @@ next
       hence "cdcl_s'\<^sup>*\<^sup>* S T"
         using st(1) by auto
       moreover have "no_step cdcl_s' T"
-        using inv_T by (metis \<open>full0 cdcl_cp T T\<close> \<open>full0 cdcl_s S T\<close> cdcl_all_inv_mes_def
+        using inv_T by (metis \<open>full0 cdcl_cp T T\<close> \<open>full0 cdcl_s S T\<close> cdcl_all_struct_inv_def
           cdcl_then_exists_cdcl_s_step full0_def n_step_cdcl_s_iff_no_step_cdcl_cl_cdcl_o)
       ultimately show ?thesis
         unfolding full0_def by blast
@@ -2030,7 +2030,7 @@ qed
 lemma conflict_step_cdcl_s_step:
   assumes
     "conflict S T"
-    "cdcl_all_inv_mes S"
+    "cdcl_all_struct_inv S"
   shows "\<exists>T. cdcl_s S T"
 proof -
   obtain U where "full0 cdcl_cp S U"
@@ -2043,11 +2043,11 @@ qed
 lemma decide_step_cdcl_s_step:
   assumes
     "decide S T"
-    "cdcl_all_inv_mes S"
+    "cdcl_all_struct_inv S"
   shows "\<exists>T. cdcl_s S T"
 proof -
   obtain U where "full0 cdcl_cp T U"
-    using cdcl_cp_normalized_element_all_inv by (meson assms(1) assms(2) cdcl_all_inv_mes_inv
+    using cdcl_cp_normalized_element_all_inv by (meson assms(1) assms(2) cdcl_all_struct_inv_inv
       cdcl_cp_normalized_element_all_inv decide other)
   thus ?thesis
     by (metis assms cdcl_cp_normalized_element_all_inv cdcl_s.conflict' decide full0_unfold other')
@@ -2270,7 +2270,7 @@ qed
 
 lemma no_step_cdcl_s'_no_ste_cdcl_fw_cp:
   assumes
-    "cdcl_all_inv_mes S"
+    "cdcl_all_struct_inv S"
     "conflicting S = C_True"
     "no_step cdcl_s' S"
   shows "no_step cdcl_fw_cp S"
@@ -2313,7 +2313,7 @@ qed
 
 lemma conflicting_true_no_step_s'_without_decide_no_step_cdcl_fw_cp:
   assumes
-    inv: "cdcl_all_inv_mes S" and
+    inv: "cdcl_all_struct_inv S" and
     n_s: "no_step cdcl_s'_without_decide S"
   shows "no_step cdcl_fw_cp S"
 proof (rule ccontr)
@@ -2327,8 +2327,8 @@ proof (rule ccontr)
     next
       case propagate'
       moreover
-        have "cdcl_all_inv_mes T"
-          using inv by (meson local.propagate' rtranclp_cdcl_all_inv_mes_inv
+        have "cdcl_all_struct_inv T"
+          using inv by (meson local.propagate' rtranclp_cdcl_all_struct_inv_inv
             rtranclp_propagate_is_rtranclp_cdcl tranclp_into_rtranclp)
         then obtain U where "full0 cdcl_cp T U"
           using cdcl_cp_normalized_element_all_inv by auto
@@ -2355,7 +2355,7 @@ lemma conflicting_not_true_rtranclp_cdcl_fw_cp_no_step_cdcl_bj:
 lemma conflicting_true_full0_cdcl_fw_cp_iff_full0_cdcl_s'_without_decode:
   assumes
     confl: "conflicting S = C_True" and
-    inv: "cdcl_all_inv_mes S"
+    inv: "cdcl_all_struct_inv S"
   shows
     "full0 cdcl_fw_cp S V \<longleftrightarrow> full0 cdcl_s'_without_decide S V" (is "?fw \<longleftrightarrow> ?s'")
 proof
@@ -2427,7 +2427,7 @@ next
     unfolding full0_def by auto
   then have "cdcl\<^sup>*\<^sup>* S V"
     using rtranclp_cdcl_s'_without_decide_rtranclp_cdcl st by blast
-  then have inv_V: "cdcl_all_inv_mes V" using inv rtranclp_cdcl_all_inv_mes_inv by blast
+  then have inv_V: "cdcl_all_struct_inv V" using inv rtranclp_cdcl_all_struct_inv_inv by blast
   then have n_s_cp_V: "no_step cdcl_cp V"
     using cdcl_cp_normalized_element_all_inv[of V] full0_fullI[of cdcl_cp V] n_s
     conflict'_without_decide conflicting_true_no_step_s'_without_decide_no_step_cdcl_fw_cp
@@ -2442,8 +2442,8 @@ next
       moreover
         then have "cdcl\<^sup>+\<^sup>+ V W'"
           using tranclp_mono[of cdcl_bj cdcl] cdcl.other cdcl_o.bj unfolding full_def by blast
-        then have "cdcl_all_inv_mes W'"
-          by (meson inv_V rtranclp_cdcl_all_inv_mes_inv tranclp_into_rtranclp)
+        then have "cdcl_all_struct_inv W'"
+          by (meson inv_V rtranclp_cdcl_all_struct_inv_inv tranclp_into_rtranclp)
         then obtain X where "full0 cdcl_cp W' X"
           using cdcl_cp_normalized_element_all_inv by blast
       ultimately show False
@@ -2467,8 +2467,8 @@ next
     qed fast+
   moreover
     then have "cdcl\<^sup>*\<^sup>* S V" using rtranclp_cdcl_fw_cp_rtranclp_cdcl by blast
-    then have "cdcl_all_inv_mes V"
-      using inv rtranclp_cdcl_all_inv_mes_inv by blast
+    then have "cdcl_all_struct_inv V"
+      using inv rtranclp_cdcl_all_struct_inv_inv by blast
     then have "no_step cdcl_fw_cp V"
       using conflicting_true_no_step_s'_without_decide_no_step_cdcl_fw_cp s'
       unfolding full0_def by blast
@@ -2478,7 +2478,7 @@ qed
 lemma conflicting_true_full_cdcl_fw_cp_iff_full_cdcl_s'_without_decode:
   assumes
     confl: "conflicting S = C_True" and
-    inv: "cdcl_all_inv_mes S"
+    inv: "cdcl_all_struct_inv S"
   shows
     "full cdcl_fw_cp S V \<longleftrightarrow> full cdcl_s'_without_decide S V"
 proof -
@@ -2492,7 +2492,7 @@ qed
 lemma conflicting_true_full_cdcl_fw_cp_imp_full_cdcl_s'_without_decode:
   assumes
     fw: "full cdcl_fw_cp S V" and
-    inv: "cdcl_all_inv_mes S"
+    inv: "cdcl_all_struct_inv S"
   shows
     "full cdcl_s'_without_decide S V"
 proof -
@@ -2575,12 +2575,12 @@ lemma after_cdcl_s'_without_decide_no_step_cdcl_cp:
   using assms by (induction rule: cdcl_s'_without_decide.induct) (auto simp: full_def full0_def)
 
 lemma no_step_cdcl_s'_without_decide_no_step_cdcl_cp:
-  "cdcl_all_inv_mes S \<Longrightarrow> no_step cdcl_s'_without_decide S \<Longrightarrow> no_step cdcl_cp S"
+  "cdcl_all_struct_inv S \<Longrightarrow> no_step cdcl_s'_without_decide S \<Longrightarrow> no_step cdcl_cp S"
   by (simp add: conflicting_true_no_step_s'_without_decide_no_step_cdcl_fw_cp
     no_step_cdcl_fw_cp_no_step_cdcl_cp)
 
 lemma after_cdcl_s'_w_no_step_cdcl_cp:
-  assumes "cdcl_s'_w S T" and "cdcl_all_inv_mes S"
+  assumes "cdcl_s'_w S T" and "cdcl_all_struct_inv S"
   shows "no_step cdcl_cp T"
   using assms
 proof (induction rule: cdcl_s'_w.induct)
@@ -2593,14 +2593,14 @@ next
     then have "cdcl\<^sup>*\<^sup>* S U"
       using rtranclp_cdcl_s'_without_decide_rtranclp_cdcl[of T U] cdcl.other[of S T] cdcl_o.decide
       unfolding full0_def by auto
-    then have "cdcl_all_inv_mes U"
-      using decide'.prems rtranclp_cdcl_all_inv_mes_inv by blast
+    then have "cdcl_all_struct_inv U"
+      using decide'.prems rtranclp_cdcl_all_struct_inv_inv by blast
   ultimately show ?case
     using no_step_cdcl_s'_without_decide_no_step_cdcl_cp unfolding full0_def by blast
 qed
 
 lemma rtranclp_cdcl_s'_w_no_step_cdcl_cp_or_eq:
-  assumes "cdcl_s'_w\<^sup>*\<^sup>* S T" and "cdcl_all_inv_mes S"
+  assumes "cdcl_s'_w\<^sup>*\<^sup>* S T" and "cdcl_all_struct_inv S"
   shows "S = T \<or> no_step cdcl_cp T"
   using assms
 proof (induction rule: rtranclp_induct)
@@ -2608,14 +2608,14 @@ proof (induction rule: rtranclp_induct)
   then show ?case by simp
 next
   case (step T U)
-  moreover have "cdcl_all_inv_mes T"
-    using rtranclp_cdcl_s'_w_rtranclp_cdcl[of S U] assms(2) rtranclp_cdcl_all_inv_mes_inv
+  moreover have "cdcl_all_struct_inv T"
+    using rtranclp_cdcl_s'_w_rtranclp_cdcl[of S U] assms(2) rtranclp_cdcl_all_struct_inv_inv
     rtranclp_cdcl_s'_w_rtranclp_cdcl step.hyps(1) by blast
   ultimately show ?case using after_cdcl_s'_w_no_step_cdcl_cp by fast
 qed
 
 lemma rtranclp_cdcl_fw_s'_no_step_cdcl_cp_or_eq:
-  assumes "cdcl_fw_s\<^sup>*\<^sup>* S T" and "cdcl_all_inv_mes S"
+  assumes "cdcl_fw_s\<^sup>*\<^sup>* S T" and "cdcl_all_struct_inv S"
   shows "S = T \<or> no_step cdcl_cp T"
   using assms
 proof (induction rule: rtranclp_induct)
@@ -2623,8 +2623,8 @@ proof (induction rule: rtranclp_induct)
   then show ?case by simp
 next
   case (step T U)
-  moreover have "cdcl_all_inv_mes T"
-    using rtranclp_cdcl_fw_s_rtranclp_cdcl[of S U] assms(2) rtranclp_cdcl_all_inv_mes_inv
+  moreover have "cdcl_all_struct_inv T"
+    using rtranclp_cdcl_fw_s_rtranclp_cdcl[of S U] assms(2) rtranclp_cdcl_all_struct_inv_inv
     rtranclp_cdcl_s'_w_rtranclp_cdcl step.hyps(1) by (meson rtranclp_cdcl_fw_s_rtranclp_cdcl)
   ultimately show ?case
     using after_cdcl_s'_w_no_step_cdcl_cp by (metis (full_types) cdcl_fw_s.simps full0_def
@@ -2632,7 +2632,7 @@ next
 qed
 
 lemma no_step_cdcl_s'_without_decide_no_step_cdcl_bj:
-  assumes "no_step cdcl_s'_without_decide S" and inv: "cdcl_all_inv_mes S"
+  assumes "no_step cdcl_s'_without_decide S" and inv: "cdcl_all_struct_inv S"
   shows "no_step cdcl_bj S"
 proof (rule ccontr)
   assume "\<not> ?thesis"
@@ -2644,8 +2644,8 @@ proof (rule ccontr)
     then have "cdcl\<^sup>*\<^sup>* S T'"
       using rtranclp_mono[of cdcl_bj cdcl] cdcl.other cdcl_o.bj tranclp_into_rtranclp[of cdcl_bj]
       unfolding full_def by (metis (full_types) predicate2D predicate2I)
-    then have "cdcl_all_inv_mes T'"
-      using inv  rtranclp_cdcl_all_inv_mes_inv by blast
+    then have "cdcl_all_struct_inv T'"
+      using inv  rtranclp_cdcl_all_struct_inv_inv by blast
     then obtain U where "full0 cdcl_cp T' U"
       using cdcl_cp_normalized_element_all_inv by blast
   moreover have "no_step cdcl_cp S"
@@ -2655,29 +2655,29 @@ proof (rule ccontr)
 qed
 
 lemma cdcl_s'_w_no_step_cdcl_bj:
-  assumes "cdcl_s'_w S T" and "cdcl_all_inv_mes S"
+  assumes "cdcl_s'_w S T" and "cdcl_all_struct_inv S"
   shows "no_step cdcl_bj T"
   using assms apply induction
-    using rtranclp_cdcl_s'_without_decide_rtranclp_cdcl rtranclp_cdcl_all_inv_mes_inv
+    using rtranclp_cdcl_s'_without_decide_rtranclp_cdcl rtranclp_cdcl_all_struct_inv_inv
     no_step_cdcl_s'_without_decide_no_step_cdcl_bj unfolding full_def
     apply (meson tranclp_into_rtranclp)
-  using rtranclp_cdcl_s'_without_decide_rtranclp_cdcl rtranclp_cdcl_all_inv_mes_inv
+  using rtranclp_cdcl_s'_without_decide_rtranclp_cdcl rtranclp_cdcl_all_struct_inv_inv
     no_step_cdcl_s'_without_decide_no_step_cdcl_bj unfolding full0_def
   by (meson cdcl_fw_restart_cdcl fw_r_decide)
 
 lemma rtranclp_cdcl_s'_w_no_step_cdcl_bj_or_eq:
-  assumes "cdcl_s'_w\<^sup>*\<^sup>* S T" and "cdcl_all_inv_mes S"
+  assumes "cdcl_s'_w\<^sup>*\<^sup>* S T" and "cdcl_all_struct_inv S"
   shows "S = T \<or> no_step cdcl_bj T"
   using assms apply induction
     apply simp
-  using rtranclp_cdcl_s'_w_rtranclp_cdcl rtranclp_cdcl_all_inv_mes_inv
+  using rtranclp_cdcl_s'_w_rtranclp_cdcl rtranclp_cdcl_all_struct_inv_inv
     cdcl_s'_w_no_step_cdcl_bj by meson
 
 lemma rtranclp_cdcl_s'_no_step_cdcl_s'_without_decide_decomp_into_cdcl_fw:
   assumes
     "cdcl_s'\<^sup>*\<^sup>* R V" and
     "conflicting R = C_True" and
-    inv: "cdcl_all_inv_mes R"
+    inv: "cdcl_all_struct_inv R"
   shows "(cdcl_fw_s\<^sup>*\<^sup>* R V \<and> conflicting V = C_True)
   \<or> (cdcl_fw_s\<^sup>*\<^sup>* R V \<and> conflicting V \<noteq> C_True \<and> no_step cdcl_bj V)
   \<or> (\<exists>S T U. cdcl_fw_s\<^sup>*\<^sup>* R S \<and> no_step cdcl_fw_cp S \<and> decide S T
@@ -3124,7 +3124,7 @@ qed
 lemma rtranclp_cdcl_fw_s_rtranclp_cdcl_s':
   assumes
     "cdcl_fw_s\<^sup>*\<^sup>* R V" and
-    inv: "cdcl_all_inv_mes R"
+    inv: "cdcl_all_struct_inv R"
   shows "cdcl_s'\<^sup>*\<^sup>* R V"
   using assms(1)
 proof induction
@@ -3132,8 +3132,8 @@ proof induction
   thus ?case by simp
 next
   case (step S T) note st = this(1) and fw = this(2) and IH = this(3)
-  have "cdcl_all_inv_mes S"
-    using inv rtranclp_cdcl_all_inv_mes_inv rtranclp_cdcl_fw_s_rtranclp_cdcl st by blast
+  have "cdcl_all_struct_inv S"
+    using inv rtranclp_cdcl_all_struct_inv_inv rtranclp_cdcl_fw_s_rtranclp_cdcl st by blast
   from fw show ?case
     proof (cases rule: cdcl_fw_s_cases)
       case fw_s_cp
@@ -3158,7 +3158,7 @@ next
             using f5 by (metis (no_types) cdcl_fw_s.simps rtranclp_unfold st
               tranclp_unfold_end)
           then show ?thesis
-            using f2 a1 by (metis (no_types) \<open>cdcl_all_inv_mes S\<close>
+            using f2 a1 by (metis (no_types) \<open>cdcl_all_struct_inv S\<close>
               conflicting_true_full_cdcl_fw_cp_imp_full_cdcl_s'_without_decode
               rtranclp_cdcl_s'_without_decide_rtranclp_cdcl_s' rtranclp_unfold)
         qed
@@ -3167,21 +3167,21 @@ next
       moreover then have "conflicting S' = C_True"
         by auto
       ultimately have "full0 cdcl_s'_without_decide S' T"
-        by (meson \<open>cdcl_all_inv_mes S\<close> cdcl_fw_restart_cdcl fw_r_decide rtranclp_cdcl_all_inv_mes_inv
+        by (meson \<open>cdcl_all_struct_inv S\<close> cdcl_fw_restart_cdcl fw_r_decide rtranclp_cdcl_all_struct_inv_inv
           conflicting_true_full0_cdcl_fw_cp_iff_full0_cdcl_s'_without_decode)
       then have a1: "cdcl_s'\<^sup>*\<^sup>* S' T"
         unfolding full0_def by (metis (full_types) rtranclp_cdcl_s'_without_decide_rtranclp_cdcl_s')
       have "cdcl_fw_s\<^sup>*\<^sup>* S T"
         using fw by blast
       then have "cdcl_s'\<^sup>*\<^sup>* S T"
-        using decide_rtranclp_cdcl_s'_rtranclp_cdcl_s' a1 by (metis \<open>cdcl_all_inv_mes S\<close> dec
+        using decide_rtranclp_cdcl_s'_rtranclp_cdcl_s' a1 by (metis \<open>cdcl_all_struct_inv S\<close> dec
           n_S no_step_cdcl_fw_cp_no_step_cdcl_cp rtranclp_cdcl_fw_s'_no_step_cdcl_cp_or_eq)
       then show ?thesis using IH by auto
     qed
 qed
 
 lemma rtranclp_cdcl_fw_s_distinct_mset_clauses:
-  assumes invR: "cdcl_all_inv_mes R" and
+  assumes invR: "cdcl_all_struct_inv R" and
   st: "cdcl_fw_s\<^sup>*\<^sup>* R S" and
   dist: "distinct_mset (clauses R)" and
   R: "trail R = []"
@@ -3192,7 +3192,7 @@ lemma rtranclp_cdcl_fw_s_distinct_mset_clauses:
 
 lemma no_step_cdcl_s'_no_step_cdcl_fw_s:
   assumes
-    inv: "cdcl_all_inv_mes R" and s': "no_step cdcl_s' R"
+    inv: "cdcl_all_struct_inv R" and s': "no_step cdcl_s' R"
   shows "no_step cdcl_fw_s R"
 proof -
   { fix ss :: 'st
@@ -3203,8 +3203,8 @@ proof -
       ff2: "\<And>p s sa. \<not> p\<^sup>+\<^sup>+ s sa \<or> p s (ssb p s sa)"
       by (meson tranclp_unfold_begin)
     obtain ssc :: "'st \<Rightarrow> 'st" where
-      ff3: "\<And>s sa sb. (\<not> cdcl_all_inv_mes s \<or> \<not> cdcl_cp s sa \<or> cdcl_s' s (ssc s))
-        \<and> (\<not> cdcl_all_inv_mes s \<or> \<not> cdcl_o s sb \<or> cdcl_s' s (ssc s))"
+      ff3: "\<And>s sa sb. (\<not> cdcl_all_struct_inv s \<or> \<not> cdcl_cp s sa \<or> cdcl_s' s (ssc s))
+        \<and> (\<not> cdcl_all_struct_inv s \<or> \<not> cdcl_o s sb \<or> cdcl_s' s (ssc s))"
       using n_step_cdcl_s_iff_no_step_cdcl_cl_cdcl_o by moura
     then have ff4: "\<And>s. \<not> cdcl_o R s"
       using s' inv by blast
@@ -3224,31 +3224,31 @@ proof -
 qed
 
 lemma wf_cdcl_fw_cp:
-  "wf{(T, S). cdcl_all_inv_mes S \<and> cdcl_fw_cp S T}"
+  "wf{(T, S). cdcl_all_struct_inv S \<and> cdcl_fw_cp S T}"
   using wf_tranclp_cdcl_fw by (rule wf_subset) (auto simp: cdcl_fw_cp_tranclp_cdcl_fw)
 
 lemma wf_cdcl_fw_s:
-  "wf{(T, S). cdcl_all_inv_mes S \<and> cdcl_fw_s S T}"
+  "wf{(T, S). cdcl_all_struct_inv S \<and> cdcl_fw_s S T}"
   using wf_tranclp_cdcl_fw by (rule wf_subset) (auto simp add: cdcl_fw_s_tranclp_cdcl_fw)
 
 lemma cdcl_fw_cp_obtain_normal_form:
-  assumes inv: "cdcl_all_inv_mes R"
+  assumes inv: "cdcl_all_struct_inv R"
   obtains S where "full0 cdcl_fw_cp R S"
 proof -
-  obtain S where "full0 (\<lambda>S T. cdcl_all_inv_mes S \<and> cdcl_fw_cp S T) R S"
+  obtain S where "full0 (\<lambda>S T. cdcl_all_struct_inv S \<and> cdcl_fw_cp S T) R S"
     using wf_exists_normal_form_full0[OF wf_cdcl_fw_cp] by blast
   then have
-    st: "(\<lambda>S T. cdcl_all_inv_mes S \<and> cdcl_fw_cp S T)\<^sup>*\<^sup>* R S" and
-    n_s: "no_step (\<lambda>S T. cdcl_all_inv_mes S \<and> cdcl_fw_cp S T) S"
+    st: "(\<lambda>S T. cdcl_all_struct_inv S \<and> cdcl_fw_cp S T)\<^sup>*\<^sup>* R S" and
+    n_s: "no_step (\<lambda>S T. cdcl_all_struct_inv S \<and> cdcl_fw_cp S T) S"
     unfolding full0_def by blast+
   have "cdcl_fw_cp\<^sup>*\<^sup>* R S"
     using st by induction auto
   moreover
-    have "cdcl_all_inv_mes S"
+    have "cdcl_all_struct_inv S"
       using st inv
       apply (induction rule: rtranclp_induct)
         apply simp
-      by (meson r_into_rtranclp rtranclp_cdcl_all_inv_mes_inv rtranclp_cdcl_fw_cp_rtranclp_cdcl)
+      by (meson r_into_rtranclp rtranclp_cdcl_all_struct_inv_inv rtranclp_cdcl_fw_cp_rtranclp_cdcl)
     then have "no_step cdcl_fw_cp S"
       using n_s by auto
   ultimately show ?thesis
@@ -3257,7 +3257,7 @@ qed
 
 lemma no_step_cdcl_fw_s_no_step_cdcl_s':
   assumes
-    inv: "cdcl_all_inv_mes R" and
+    inv: "cdcl_all_struct_inv R" and
     confl: "conflicting R = C_True" and
     n_s: "no_step cdcl_fw_s R"
   shows "no_step cdcl_s' R"
@@ -3273,8 +3273,8 @@ proof (rule ccontr)
       then show False using n_s by blast
     next
       case (decide' R')
-      then have "cdcl_all_inv_mes R'"
-        using inv cdcl_all_inv_mes_inv cdcl.other cdcl_o.decide by meson
+      then have "cdcl_all_struct_inv R'"
+        using inv cdcl_all_struct_inv_inv cdcl.other cdcl_o.decide by meson
       then obtain R'' where "full0 cdcl_fw_cp R' R''"
         using cdcl_fw_cp_obtain_normal_form by blast
       moreover have "no_step cdcl_fw_cp R"
@@ -3321,29 +3321,29 @@ qed
 lemma full0_cdcl_s'_full0_cdcl_fw_restart:
   assumes
     "conflicting R = C_True" and
-    inv: "cdcl_all_inv_mes R"
+    inv: "cdcl_all_struct_inv R"
   shows "full0 cdcl_s' R V \<longleftrightarrow> full0 cdcl_fw_s R V" (is "?s' \<longleftrightarrow> ?fw")
 proof
   assume ?s'
   then have "cdcl_s'\<^sup>*\<^sup>* R V" unfolding full0_def by blast
-  have "cdcl_all_inv_mes V"
-    using \<open>cdcl_s'\<^sup>*\<^sup>* R V\<close> inv rtranclp_cdcl_all_inv_mes_inv rtranclp_cdcl_s'_rtranclp_cdcl by blast
+  have "cdcl_all_struct_inv V"
+    using \<open>cdcl_s'\<^sup>*\<^sup>* R V\<close> inv rtranclp_cdcl_all_struct_inv_inv rtranclp_cdcl_s'_rtranclp_cdcl by blast
   then have n_s: "no_step cdcl_fw_s V"
     using no_step_cdcl_s'_no_step_cdcl_fw_s by (meson \<open>full0 cdcl_s' R V\<close> full0_def)
   have n_s_bj: "no_step cdcl_bj V"
-    by (metis \<open>cdcl_all_inv_mes V\<close> \<open>full0 cdcl_s' R V\<close> bj full0_def
+    by (metis \<open>cdcl_all_struct_inv V\<close> \<open>full0 cdcl_s' R V\<close> bj full0_def
       n_step_cdcl_s_iff_no_step_cdcl_cl_cdcl_o)
   have n_s_cp: "no_step cdcl_fw_cp V"
     proof -
       { fix ss :: 'st
         obtain ssa :: "'st \<Rightarrow> 'st" where
-          ff1: "\<forall>s. \<not> cdcl_all_inv_mes s \<or> cdcl_s'_without_decide s (ssa s) \<or> no_step cdcl_fw_cp s"
+          ff1: "\<forall>s. \<not> cdcl_all_struct_inv s \<or> cdcl_s'_without_decide s (ssa s) \<or> no_step cdcl_fw_cp s"
           using conflicting_true_no_step_s'_without_decide_no_step_cdcl_fw_cp by moura
         have "(\<forall>p s sa. \<not> full0 p (s::'st) sa \<or> p\<^sup>*\<^sup>* s sa \<and> no_step p sa)" and
           "(\<forall>p s sa. (\<not> p\<^sup>*\<^sup>* (s::'st) sa \<or> (\<exists>s. p sa s)) \<or> full0 p s sa)"
           by (meson full0_def)+
         then have "\<not> cdcl_fw_cp V ss"
-          using ff1 by (metis (no_types) \<open>cdcl_all_inv_mes V\<close> \<open>full0 cdcl_s' R V\<close> cdcl_s'.simps
+          using ff1 by (metis (no_types) \<open>cdcl_all_struct_inv V\<close> \<open>full0 cdcl_s' R V\<close> cdcl_s'.simps
             cdcl_s'_without_decide.cases) }
       then show ?thesis
         by blast
@@ -3401,7 +3401,7 @@ next
   assume ?fw
   then have "cdcl\<^sup>*\<^sup>* R V" using rtranclp_mono[of cdcl_fw_s "cdcl\<^sup>*\<^sup>*"]
     cdcl_fw_s_rtranclp_cdcl unfolding full0_def by auto
-  then have inv': "cdcl_all_inv_mes V" using inv rtranclp_cdcl_all_inv_mes_inv by blast
+  then have inv': "cdcl_all_struct_inv V" using inv rtranclp_cdcl_all_struct_inv_inv by blast
   have "cdcl_s'\<^sup>*\<^sup>* R V"
     using \<open>?fw\<close> by (simp add: full0_def inv rtranclp_cdcl_fw_s_rtranclp_cdcl_s')
   moreover have "no_step cdcl_s' V"
@@ -3424,7 +3424,7 @@ qed
 lemma full0_cdcl_s_full0_cdcl_fw:
   assumes
     "conflicting R = C_True" and
-    inv: "cdcl_all_inv_mes R"
+    inv: "cdcl_all_struct_inv R"
   shows "full0 cdcl_s R V \<longleftrightarrow> full0 cdcl_fw_s R V" (is "?s' \<longleftrightarrow> ?fw")
   by (simp add: assms(1) full0_cdcl_s'_full0_cdcl_fw_restart full0_cdcl_s_iff_full0_cdcl_s' inv)
 
@@ -3435,8 +3435,8 @@ lemma full_cdcl_fw_s_normal_forms':
   shows "(conflicting S' = C_Clause {#} \<and> unsatisfiable (set_mset N))
     \<or> (conflicting S' = C_True \<and> trail S' \<Turnstile>asm N \<and> satisfiable (set_mset N))"
 proof -
-  have "cdcl_all_inv_mes (init_state N)"
-    using no_d unfolding cdcl_all_inv_mes_def by auto
+  have "cdcl_all_struct_inv (init_state N)"
+    using no_d unfolding cdcl_all_struct_inv_def by auto
   moreover have "conflicting (init_state N) = C_True"
     by auto
   ultimately show ?thesis
@@ -3500,23 +3500,23 @@ lemma cdcl_with_restart\<^sub>C\<^sub>W_increasing_number:
 lemma "full cdcl_fw_s S T \<Longrightarrow> cdcl_with_restart\<^sub>C\<^sub>W (S, n) (T, Suc n)"
   using restart_full by blast
 
-lemma cdcl_all_inv_mes_learned_clss_bound:
-  assumes inv: "cdcl_all_inv_mes S"
+lemma cdcl_all_struct_inv_learned_clss_bound:
+  assumes inv: "cdcl_all_struct_inv S"
   shows "set_mset (learned_clss S) \<subseteq> build_all_simple_clss (atms_of_mu (init_clss S))"
 proof
   fix C
   assume C: "C \<in> set_mset (learned_clss S)"
   have "distinct_mset C"
-    using C inv unfolding cdcl_all_inv_mes_def distinct_cdcl_state_def distinct_mset_set_def by auto
+    using C inv unfolding cdcl_all_struct_inv_def distinct_cdcl_state_def distinct_mset_set_def by auto
   moreover have "\<not>tautology C"
-    using C inv unfolding cdcl_all_inv_mes_def cdcl_learned_clause_def by auto
+    using C inv unfolding cdcl_all_struct_inv_def cdcl_learned_clause_def by auto
   moreover
     have "atms_of C \<subseteq> atms_of_mu (learned_clss S)"
       using C by auto
     then have "atms_of C \<subseteq> atms_of_mu (init_clss S)"
-    using inv  unfolding cdcl_all_inv_mes_def no_strange_atm_def by force
+    using inv  unfolding cdcl_all_struct_inv_def no_strange_atm_def by force
   moreover have "finite (atms_of_mu (init_clss S))"
-    using inv unfolding cdcl_all_inv_mes_def by auto
+    using inv unfolding cdcl_all_struct_inv_def by auto
   ultimately show "C \<in> build_all_simple_clss (atms_of_mu (init_clss S))"
     using distinct_mset_not_tautology_implies_in_build_all_simple_clss build_all_simple_clss_mono
     by blast
@@ -3560,12 +3560,12 @@ lemma cdcl_with_restart\<^sub>C\<^sub>W_init_clss:
   using cdcl_with_restart\<^sub>C\<^sub>W_rtranclp_cdcl rtranclp_cdcl_init_clss by blast
 
 lemma
-  "wf {(T, S). cdcl_all_inv_mes (fst S) \<and> cdcl_with_restart\<^sub>C\<^sub>W S T}"
+  "wf {(T, S). cdcl_all_struct_inv (fst S) \<and> cdcl_with_restart\<^sub>C\<^sub>W S T}"
 proof (rule ccontr)
   assume "\<not> ?thesis"
     then obtain g where
     g: "\<And>i. cdcl_with_restart\<^sub>C\<^sub>W (g i) (g (Suc i))" and
-    inv: "\<And>i. cdcl_all_inv_mes (fst (g i))"
+    inv: "\<And>i. cdcl_all_struct_inv (fst (g i))"
     unfolding wf_iff_no_infinite_down_chain by fast
   { fix i
     have "init_clss (fst (g i)) = init_clss (fst (g 0))"
@@ -3575,7 +3575,7 @@ proof (rule ccontr)
     } note init_g = this
   let ?S = "g 0"
   have "finite (atms_of_mu (init_clss (fst ?S)))"
-    using inv unfolding cdcl_all_inv_mes_def by auto
+    using inv unfolding cdcl_all_struct_inv_def by auto
   have "\<And>i. snd (g i) < snd (g (i+1))"
     by (metis Suc_eq_plus1 Suc_le_lessD add.commute cdcl_with_restart\<^sub>C\<^sub>W_increasing_number g
       less_or_eq_imp_le)
@@ -3609,8 +3609,8 @@ proof (rule ccontr)
     using g[of j] H[of "Suc j"] by (force simp: cdcl_with_restart\<^sub>C\<^sub>W.simps full_def)
   have "cdcl_fw_s\<^sup>*\<^sup>* (fst (g j)) T"
     using cdcl_fw_s relpowp_imp_rtranclp by metis
-  then have "cdcl_all_inv_mes T"
-    using inv[of j]  rtranclp_cdcl_all_inv_mes_inv rtranclp_cdcl_fw_s_rtranclp_cdcl by blast
+  then have "cdcl_all_struct_inv T"
+    using inv[of j]  rtranclp_cdcl_all_struct_inv_inv rtranclp_cdcl_fw_s_rtranclp_cdcl by blast
   moreover have "card (set_mset (learned_clss T)) - card (set_mset (learned_clss (fst (g j))))
       > card (build_all_simple_clss (atms_of_mu (init_clss (fst ?S))))"
     by (smt Suc_leI \<open>f (snd (g j)) < m\<close> dual_order.trans f j le_less_linear less_imp_le m
@@ -3625,12 +3625,12 @@ proof (rule ccontr)
     then have "init_clss (fst ?S) = init_clss T"
       using init_g[of j] by auto
   ultimately show False
-    using cdcl_all_inv_mes_learned_clss_bound by (metis Suc_leI card_mono not_less_eq_eq
+    using cdcl_all_struct_inv_learned_clss_bound by (metis Suc_leI card_mono not_less_eq_eq
       build_all_simple_clss_finite)
 qed
 
 lemma cdcl_with_restart\<^sub>C\<^sub>W_distinct_mset_clauses:
-  assumes invR: "cdcl_all_inv_mes (fst R)" and
+  assumes invR: "cdcl_all_struct_inv (fst R)" and
   st: "cdcl_with_restart\<^sub>C\<^sub>W R S" and
   dist: "distinct_mset (clauses (fst R))" and
   R: "trail (fst R) = []"
@@ -3664,27 +3664,27 @@ lemma cdcl_s_cdcl_s_invariant:
   assumes
    cdcl: "cdcl_s S T" and
    inv_s: "cdcl_s_invariant S" and
-   inv: "cdcl_all_inv_mes S"
+   inv: "cdcl_all_struct_inv S"
   shows
     "cdcl_s_invariant T"
-  unfolding cdcl_s_invariant_def cdcl_all_inv_mes_def apply standard
+  unfolding cdcl_s_invariant_def cdcl_all_struct_inv_def apply standard
     apply (rule cdcl_s_ex_lit_of_max_level[of S])
-    using assms unfolding cdcl_s_invariant_def cdcl_all_inv_mes_def apply auto[7]
+    using assms unfolding cdcl_s_invariant_def cdcl_all_struct_inv_def apply auto[7]
   apply standard
     using cdcl cdcl_s_not_non_negated_init_clss apply blast
   apply (rule cdcl_s_no_smaller_confl_inv)
-  using assms unfolding cdcl_s_invariant_def cdcl_all_inv_mes_def by auto
+  using assms unfolding cdcl_s_invariant_def cdcl_all_struct_inv_def by auto
 
 lemma rtranclp_cdcl_s_cdcl_s_invariant:
   assumes
    cdcl: "cdcl_s\<^sup>*\<^sup>* S T" and
    inv_s: "cdcl_s_invariant S" and
-   inv: "cdcl_all_inv_mes S"
+   inv: "cdcl_all_struct_inv S"
   shows
     "cdcl_s_invariant T"
   using assms apply (induction)
     apply simp
-  using cdcl_s_cdcl_s_invariant rtranclp_cdcl_all_inv_mes_inv rtranclp_cdcl_s_rtranclp_cdcl by blast
+  using cdcl_s_cdcl_s_invariant rtranclp_cdcl_all_struct_inv_inv rtranclp_cdcl_s_rtranclp_cdcl by blast
 
 fun cut_trail_wrt_clause
   :: "'v clause \<Rightarrow> ('v, nat, 'v clause) marked_lits \<Rightarrow> ('v, nat, 'v clause) marked_lits"  where
